Reduce Target2.samplePolyCBD.eta2_loop.spec.aux lemmas to shiftDistribMask1431655765

proofs/Symcrust/Properties/SamplePolyCBD/Target2Eta2Proofs.lean
@@ -2,6 +2,7 @@ import Symcrust.Spec
 import Symcrust.Code.Funs
 import Symcrust.Brute
 import Symcrust.Properties.SamplePolyCBD.Target2Code
+import Symcrust.Properties.SamplePolyCBD.Target2HelperLemmas
 
 /-!
 This file contains theorems about `Symcrust.Spec.samplePolyCBD` defined in Symcrust.Spec.Spec.lean.
@@ -16,7 +17,11 @@ This file contains theorems about `Symcrust.Spec.samplePolyCBD` defined in Symcr
     - `⟷₂` corresponds to `Target.samplePolyCBD.eq_spec`.
     - Analogues for later portions of the verification pipeline appear in other files.
 
-  `Target2.samplePolyCBD.eta2_loop.spec` (which is the critical theorem in this file) proves `⟷₃` when `η = 2`
+  `Target2.samplePolyCBD.eta2_loop.spec` (which is the critical theorem in this file) proves `⟷₃` when `η = 2`.
+
+  **Note** although the various `Target2.samplePolyCBD.eta2_loop.spec.aux` lemmas appear to be extremely similar,
+  there are enough minor changes to the indices that appear in the arguments that there is not a convenient way
+  to combine all of these lemmas into one parameterized theorem.
 -/
 
 #setup_aeneas_simps
@@ -46,6 +51,954 @@ def Target2.samplePolyCBD.eta2_loop.inner_loop.preserves_above (pe_dst : Polynom
     Vector.getElem!_set!_ne, Vector.getElem!_set!_ne, Vector.getElem!_set!_ne, Vector.getElem!_set!_ne]
   all_goals omega
 
+lemma Fin.unfold2 {α} [AddCommMonoid α] {n : Nat} (hn : n = 2) (f : Fin n → α) :
+  ∑ x : Fin n, f x = f ⟨0, by omega⟩ + f ⟨1, by omega⟩ := by
+  rw [Finset.sum, Multiset.map, Multiset.sum, Finset.univ, Fintype.elems, Fin.fintype]
+  simp only [List.finRange, List.ofFn, Fin.foldr, hn, Fin.foldr.loop, Multiset.lift_coe, List.map_cons,
+    List.map_nil, Multiset.coe_foldr, List.foldr_cons, List.foldr_nil, add_zero, add_assoc]
+
+/-- Distributing `>>>` over `+` is not valid in general, but this lemma is true because
+    of the masks applied to `x` and `y`. -/
+lemma shiftDistribMask1431655765 {x y shift k : ℕ}
+  (hShift : shift = 4 ∨ shift = 8 ∨ shift = 12 ∨ shift = 16 ∨ shift = 20 ∨ shift = 24 ∨ shift = 28)
+  (hk : k < 4) :
+  (((x &&& 1431655765) + (y &&& 1431655765)) >>> shift).testBit k =
+  ((x &&& 1431655765) >>> shift + (y &&& 1431655765) >>> shift).testBit k := by
+  sorry
+
+theorem Target2.samplePolyCBD.eta2_loop.spec.aux0 {s : samplePolyCBDState}
+  (BVector : Vector Byte (64 * ↑s.η))
+  (hBVector : BVector = ⟨s.B.take (64 * s.η), by have := s.hB; simp; omega⟩)
+  (hs1 : ∀ j < s.i, s.pe_dst[j]! = (Target.samplePolyCBD BVector)[j]!) (hs2 : ∀ j < 256, s.i ≤ j → s.pe_dst[j]! = 0)
+  (hs3 : s.src_i * 8 = s.i * 4) (hs4 : 8 ∣ s.i) (hs5 : 4 ∣ s.src_i) (hη : s.η.val = 2)
+  (hs6 : s.i < ↑key.MLWE_POLYNOMIAL_COEFFICIENTS) (j : ℕ) (hj1 : j < s.i + 8) (hj2 : ¬j < s.i)
+  (sample_bits : BitVec (8 * (List.slice s.src_i (s.src_i + 4) s.B.toList).length))
+  (hsample_bits :
+    sample_bits =
+      (BitVec.fromLEBytes (List.slice s.src_i (s.src_i + 4) s.B.toList) &&&
+          1431655765#(8 * (List.slice s.src_i (s.src_i + 4) s.B.toList).length)) +
+        (BitVec.fromLEBytes (List.slice s.src_i (s.src_i + 4) s.B.toList) >>> 1 &&&
+          1431655765#(8 * (List.slice s.src_i (s.src_i + 4) s.B.toList).length)))
+  (hBytesToBits : ∀ i < 64 * s.η.val, ∀ j < 8, (Target.bytesToBits BVector)[8 * i + j]! = s.B[i]!.testBit j)
+  (hj3 : j = s.i) :
+  (↑↑(inner_loop.next_coefficient s.i 0 (BitVec.setWidth 32 sample_bits)).2 : ZMod 3329) =
+    ∑ x : Fin s.η.val, ↑(Target.bytesToBits BVector)[2 * s.i * s.η.val + x.val]!.toNat -
+      ∑ x : Fin s.η.val, ↑(Target.bytesToBits BVector)[2 * s.i * s.η.val + s.η.val + x.val]!.toNat := by
+  simp only [hη, Nat.mul_assoc 2 s.i 2, Nat.mul_comm s.i 2, ← Nat.mul_assoc 2 2 s.i, Nat.reduceMul,
+    Nat.mul_comm 4 s.i, ← hs3, Fin.unfold2, Nat.mul_comm s.src_i 8]
+  specialize hBytesToBits s.src_i (by scalar_tac)
+  rw [hBytesToBits 0 (by omega), hBytesToBits 1 (by omega), hBytesToBits 2 (by omega), hBytesToBits 3 (by omega)]
+  unfold inner_loop.next_coefficient
+  simp only [BitVec.ofNat_eq_ofNat, ntt.Q.eq, UScalar.ofNat_val_eq, Nat.cast_ofNat,
+    BitVec.toNat_add, BitVec.toNat_sub, Nat.reducePow, BitVec.toNat_ushiftRight, BitVec.toNat_and,
+    BitVec.toNat_setWidth, BitVec.toNat_ofNat, Nat.reduceMod, Nat.mod_add_mod]
+  olet hsample_bits_slice : sample_bits_slice := sample_bits.toNat % 4294967296 &&& 15
+  olet hs_B_byte : s_B_byte := s.B[s.src_i]!
+  replace hs_B_byte : sample_bits_slice = (s_B_byte &&& 5) + ((s_B_byte >>> 1) &&& 5) := by
+    rw [hsample_bits_slice, hsample_bits]
+    simp only [BitVec.toNat_add, BitVec.toNat_and, BitVec.toNat_ofNat,
+      BitVec.toNat_ushiftRight, Nat.mod_add_mod, BitVec.natCast_eq_ofNat, BitVec.ofNat_and,
+      Nat.cast_ofNat, BitVec.ofNat_eq_ofNat]
+    have sHB := s.hB
+    have hmin : min (s.B.size - s.src_i) 4 = 4 := by scalar_tac
+    simp only [List.slice_length, Array.length_toList, add_tsub_cancel_left]
+    olet hy : y := (BitVec.fromLEBytes (List.slice s.src_i (s.src_i + 4) s.B.toList)).toNat >>> 1
+    olet hx : x := (BitVec.fromLEBytes (List.slice s.src_i (s.src_i + 4) s.B.toList)).toNat
+    olet hx' : x' := (x &&& 1431655765 % 2 ^ (8 * min (s.B.size - s.src_i) 4))
+    olet hy' : y' := (y &&& 1431655765 % 2 ^ (8 * min (s.B.size - s.src_i) 4))
+    rw [Nat.mod_eq_of_lt] at hx' hy' <;> (try rw [hmin]; decide +native)
+    have hy'' : y' < 1431655765 + 1 := by
+      apply Nat.lt_succ_of_le
+      rw [hy']
+      exact Nat.and_le_right
+    have hx'' : x' < 1431655765 + 1 := by
+      apply Nat.lt_succ_of_le
+      rw [hx']
+      exact Nat.and_le_right
+    rw [Nat.mod_eq_of_lt, Nat.mod_eq_of_lt]
+    . rw [(by decide : 15#8 = 2#8^4 - 1#8), BitVec.and_two_pow_sub_one_eq_mod]
+      ext k hk1
+      by_cases hk2 : k < 4
+      . simp only [← BitVec.getElem!_eq_getElem, BitVec.getElem!_mod_pow2_eq _ _ _ hk2,
+          BitVec.getElem!_eq_testBit_toNat, BitVec.toNat_ofNat, Nat.reducePow, BitVec.toNat_add,
+          BitVec.toNat_and, Nat.reduceMod, BitVec.toNat_ushiftRight, Nat.mod_add_mod]
+        rw [testBitMod256 (x' + y') k (by omega), Nat.mod_eq_of_lt]
+        . apply testBitOfAdd 4 _ _ k hk2
+          . intro i hi
+            simp only [hx', hx, Nat.testBit_and, Nat.testBit_shiftRight,
+              ← BitVec.getElem!_eq_testBit_toNat, BitVec.fromLEBytes_getElem!]
+            rw [List.getElem!_slice, hs_B_byte, Array.getElem!_toList]
+            . simp_scalar
+              congr 1
+              revert i
+              decide
+            . scalar_tac
+          . intro i hi
+            simp only [hy', hy, hx, Nat.testBit_and, Nat.testBit_shiftRight,
+              ← BitVec.getElem!_eq_testBit_toNat, BitVec.fromLEBytes_getElem!]
+            rw [List.getElem!_slice, hs_B_byte, Array.getElem!_toList]
+            . simp_scalar
+              congr 1
+              revert i
+              decide
+            . scalar_tac
+        . have : (BitVec.toNat s_B_byte &&& 5) ≤ 5 := Nat.and_le_right
+          have : (BitVec.toNat s_B_byte >>> 1) &&& 5 ≤ 5 := Nat.and_le_right
+          omega
+      . have : (s_B_byte &&& 5#8) + (s_B_byte >>> 1 &&& 5#8) < 2^4 := by
+          clear hs_B_byte hBytesToBits
+          revert s_B_byte
+          decide +native -- **TODO** Once `brute` supports unbounded UScalars, `brute` should be faster
+        rw [← BitVec.getElem!_eq_getElem, ← BitVec.getElem!_eq_getElem,
+          BitVec.getElem!_mod_pow2_false _ _ _ (by omega), BitVec.getElem!_eq_testBit_toNat,
+          ← Nat.mod_eq_of_lt this]
+        simp only [BitVec.toNat_add, BitVec.toNat_and, BitVec.toNat_ofNat, Nat.reducePow,
+          Nat.reduceMod, BitVec.toNat_ushiftRight, Nat.mod_add_mod, BitVec.ofNat_eq_ofNat,
+          BitVec.toNat_pow, Nat.reduceDvd, Nat.mod_mod_of_dvd, Bool.false_eq]
+        rw [(by decide : 16 = 2^4), Nat.testBit_mod_two_pow,
+          Bool.and_eq_false_eq_eq_false_or_eq_false]
+        left
+        simp only [decide_eq_false_iff_not, not_lt]
+        omega
+    . rw [hmin]; omega
+    . rw [hmin, Nat.mod_eq_of_lt] <;> omega
+  replace hsample_bits_slice : sample_bits_slice < 16 := by
+    rw [hsample_bits_slice]
+    exact Nat.lt_succ_of_le Nat.and_le_right
+  clear hBytesToBits
+  revert s_B_byte
+  revert sample_bits_slice
+  brute
+
+theorem Target2.samplePolyCBD.eta2_loop.spec.aux1 {s : samplePolyCBDState}
+  (BVector : Vector Byte (64 * ↑s.η))
+  (hBVector : BVector = ⟨s.B.take (64 * s.η), by have := s.hB; simp; omega⟩)
+  (hs1 : ∀ j < s.i, s.pe_dst[j]! = (Target.samplePolyCBD BVector)[j]!) (hs2 : ∀ j < 256, s.i ≤ j → s.pe_dst[j]! = 0)
+  (hs3 : s.src_i * 8 = s.i * 4) (hs4 : 8 ∣ s.i) (hs5 : 4 ∣ s.src_i) (hη : s.η.val = 2)
+  (hs6 : s.i < ↑key.MLWE_POLYNOMIAL_COEFFICIENTS) (j : ℕ) (hj1 : j < s.i + 8) (hj2 : ¬j < s.i)
+  (sample_bits : BitVec (8 * (List.slice s.src_i (s.src_i + 4) s.B.toList).length))
+  (hsample_bits :
+    sample_bits =
+      (BitVec.fromLEBytes (List.slice s.src_i (s.src_i + 4) s.B.toList) &&&
+          1431655765#(8 * (List.slice s.src_i (s.src_i + 4) s.B.toList).length)) +
+        (BitVec.fromLEBytes (List.slice s.src_i (s.src_i + 4) s.B.toList) >>> 1 &&&
+          1431655765#(8 * (List.slice s.src_i (s.src_i + 4) s.B.toList).length)))
+  (hBytesToBits : ∀ i < 64 * s.η.val, ∀ j < 8, (Target.bytesToBits BVector)[8 * i + j]! = s.B[i]!.testBit j)
+  (hj3 : j = s.i + 1) :
+  (↑↑(inner_loop.next_coefficient s.i 1
+    (inner_loop.next_coefficient s.i 0 (BitVec.setWidth 32 sample_bits)).1).2 : ZMod 3329) =
+    ∑ x : Fin s.η.val, ↑(Target.bytesToBits BVector)[2 * (s.i + 1) * ↑s.η + ↑x]!.toNat -
+      ∑ x : Fin s.η.val, ↑(Target.bytesToBits BVector)[2 * (s.i + 1) * ↑s.η + ↑s.η + ↑x]!.toNat := by
+  simp only [hη, Nat.mul_assoc 2 (s.i + 1) 2, Nat.mul_comm (s.i + 1) 2, ← Nat.mul_assoc 2 2 (s.i + 1),
+    Nat.reduceMul, Nat.mul_add 4, Nat.mul_comm 4 s.i, ← hs3, Fin.unfold2, Nat.mul_comm s.src_i 8]
+  conv in 8 * s.src_i + 4 + 0 => rw [(by omega : 8 * s.src_i + 4 + 0 = 8 * s.src_i + 4)]
+  conv in 8 * s.src_i + 4 + 1 => rw [(by omega : 8 * s.src_i + 4 + 1 = 8 * s.src_i + 5)]
+  conv in 8 * s.src_i + 4 + 2 + 0 => rw [(by omega : 8 * s.src_i + 4 + 2 + 0 = 8 * s.src_i + 6)]
+  conv in 8 * s.src_i + 4 + 2 + 1 => rw [(by omega : 8 * s.src_i + 4 + 2 + 1 = 8 * s.src_i + 7)]
+  rw [hBytesToBits s.src_i (by scalar_tac) 4 (by omega),
+      hBytesToBits s.src_i (by scalar_tac) 5 (by omega),
+      hBytesToBits s.src_i (by scalar_tac) 6 (by omega),
+      hBytesToBits s.src_i (by scalar_tac) 7 (by omega)]
+  unfold inner_loop.next_coefficient
+  simp only [BitVec.ofNat_eq_ofNat, ntt.Q.eq, UScalar.ofNat_val_eq, Nat.cast_ofNat,
+    BitVec.toNat_add, BitVec.toNat_sub, Nat.reducePow, BitVec.toNat_ushiftRight, BitVec.toNat_and,
+    BitVec.toNat_setWidth, BitVec.toNat_ofNat, Nat.reduceMod, Nat.mod_add_mod]
+  olet hsample_bits_slice : sample_bits_slice := (sample_bits.toNat % 4294967296) >>> 4 &&& 15
+  olet hs_B_byte : s_B_byte := s.B[s.src_i]!
+  replace hs_B_byte : sample_bits_slice = (s_B_byte >>> 4 &&& 5) + ((s_B_byte >>> 5) &&& 5) := by
+    rw [hsample_bits_slice, hsample_bits]
+    simp only [BitVec.toNat_add, BitVec.toNat_and, BitVec.toNat_ofNat,
+      BitVec.toNat_ushiftRight, Nat.mod_add_mod, BitVec.natCast_eq_ofNat, BitVec.ofNat_and,
+      Nat.cast_ofNat, BitVec.ofNat_eq_ofNat]
+    have sHB := s.hB
+    have hmin : min (s.B.size - s.src_i) 4 = 4 := by scalar_tac
+    simp only [List.slice_length, Array.length_toList, add_tsub_cancel_left]
+    olet hy : y := (BitVec.fromLEBytes (List.slice s.src_i (s.src_i + 4) s.B.toList)).toNat >>> 1
+    olet hx : x := (BitVec.fromLEBytes (List.slice s.src_i (s.src_i + 4) s.B.toList)).toNat
+    olet hx' : x' := (x &&& 1431655765 % 2 ^ (8 * min (s.B.size - s.src_i) 4))
+    olet hy' : y' := (y &&& 1431655765 % 2 ^ (8 * min (s.B.size - s.src_i) 4))
+    rw [Nat.mod_eq_of_lt] at hx' hy' <;> (try rw [hmin]; decide +native)
+    have hy'' : y' < 1431655765 + 1 := by
+      apply Nat.lt_succ_of_le
+      rw [hy']
+      exact Nat.and_le_right
+    have hx'' : x' < 1431655765 + 1 := by
+      apply Nat.lt_succ_of_le
+      rw [hx']
+      exact Nat.and_le_right
+    rw [Nat.mod_eq_of_lt, Nat.mod_eq_of_lt]
+    . rw [(by decide : 15#8 = 2#8^4 - 1#8), BitVec.and_two_pow_sub_one_eq_mod]
+      ext k hk1
+      by_cases hk2 : k < 4
+      . simp only [← BitVec.getElem!_eq_getElem, BitVec.getElem!_mod_pow2_eq _ _ _ hk2,
+          BitVec.getElem!_eq_testBit_toNat, BitVec.toNat_ofNat, Nat.reducePow, BitVec.toNat_add,
+          BitVec.toNat_and, Nat.reduceMod, BitVec.toNat_ushiftRight, Nat.mod_add_mod]
+        rw [testBitMod256 ((x' + y') >>> 4) k (by omega), Nat.mod_eq_of_lt]
+        . rw [hx', hy', hy, shiftDistribMask1431655765 (by omega) hk2, ← hy, ← hy', ← hx']
+          apply testBitOfAdd 4 _ _ k hk2
+          . intro i hi
+            simp only [hx', hx, Nat.testBit_and, Nat.testBit_shiftRight,
+              ← BitVec.getElem!_eq_testBit_toNat, BitVec.fromLEBytes_getElem!]
+            rw [List.getElem!_slice, hs_B_byte, Array.getElem!_toList]
+            . simp_scalar
+              congr 1
+              revert i
+              decide
+            . scalar_tac
+          . intro i hi
+            simp only [hy', hy, hx, Nat.testBit_and, Nat.testBit_shiftRight,
+              ← BitVec.getElem!_eq_testBit_toNat, BitVec.fromLEBytes_getElem!]
+            by_cases hi2 : i < 3
+            . rw [(by omega : (1 + (4 + i)) / 8 = 0), (by omega : (1 + (4 + i)) % 8 = 5 + i),
+                List.getElem!_slice, hs_B_byte, Array.getElem!_toList, Nat.add_zero]
+              . congr 1
+                revert i
+                decide
+              . scalar_tac
+            . have h1 : Nat.testBit 1431655765 (4 + i) = false := by revert i; decide
+              have h2 : Nat.testBit 5 i = false := by revert i; decide
+              simp only [h1, Bool.and_false, h2]
+        . have : (BitVec.toNat s_B_byte >>> 4) &&& 5 ≤ 5 := Nat.and_le_right
+          have : (BitVec.toNat s_B_byte >>> 5) &&& 5 ≤ 5 := Nat.and_le_right
+          omega
+      . have : (s_B_byte >>> 4 &&& 5#8) + (s_B_byte >>> 5 &&& 5#8) < 2^4 := by
+          clear hs_B_byte hBytesToBits
+          revert s_B_byte
+          decide +native -- **TODO** Once `brute` supports unbounded UScalars, `brute` should be faster
+        rw [← BitVec.getElem!_eq_getElem, ← BitVec.getElem!_eq_getElem,
+          BitVec.getElem!_mod_pow2_false _ _ _ (by omega), BitVec.getElem!_eq_testBit_toNat,
+          ← Nat.mod_eq_of_lt this]
+        simp only [BitVec.toNat_add, BitVec.toNat_and, BitVec.toNat_ofNat, Nat.reducePow,
+          Nat.reduceMod, BitVec.toNat_ushiftRight, Nat.mod_add_mod, BitVec.ofNat_eq_ofNat,
+          BitVec.toNat_pow, Nat.reduceDvd, Nat.mod_mod_of_dvd, Bool.false_eq]
+        rw [(by decide : 16 = 2^4), Nat.testBit_mod_two_pow,
+          Bool.and_eq_false_eq_eq_false_or_eq_false]
+        left
+        simp only [decide_eq_false_iff_not, not_lt]
+        omega
+    . rw [hmin]; omega
+    . rw [hmin, Nat.mod_eq_of_lt] <;> omega
+  replace hsample_bits_slice : sample_bits_slice < 16 := by
+    rw [hsample_bits_slice]
+    exact Nat.lt_succ_of_le Nat.and_le_right
+  clear hBytesToBits
+  revert s_B_byte
+  revert sample_bits_slice
+  brute
+
+theorem Target2.samplePolyCBD.eta2_loop.spec.aux2 {s : samplePolyCBDState}
+  (BVector : Vector Byte (64 * ↑s.η))
+  (hBVector : BVector = ⟨s.B.take (64 * s.η), by have := s.hB; simp; omega⟩)
+  (hs1 : ∀ j < s.i, s.pe_dst[j]! = (Target.samplePolyCBD BVector)[j]!) (hs2 : ∀ j < 256, s.i ≤ j → s.pe_dst[j]! = 0)
+  (hs3 : s.src_i * 8 = s.i * 4) (hs4 : 8 ∣ s.i) (hs5 : 4 ∣ s.src_i) (hη : s.η.val = 2)
+  (hs6 : s.i < ↑key.MLWE_POLYNOMIAL_COEFFICIENTS) (j : ℕ) (hj1 : j < s.i + 8) (hj2 : ¬j < s.i)
+  (sample_bits : BitVec (8 * (List.slice s.src_i (s.src_i + 4) s.B.toList).length))
+  (hsample_bits :
+    sample_bits =
+      (BitVec.fromLEBytes (List.slice s.src_i (s.src_i + 4) s.B.toList) &&&
+          1431655765#(8 * (List.slice s.src_i (s.src_i + 4) s.B.toList).length)) +
+        (BitVec.fromLEBytes (List.slice s.src_i (s.src_i + 4) s.B.toList) >>> 1 &&&
+          1431655765#(8 * (List.slice s.src_i (s.src_i + 4) s.B.toList).length)))
+  (hBytesToBits : ∀ i < 64 * s.η.val, ∀ j < 8, (Target.bytesToBits BVector)[8 * i + j]! = s.B[i]!.testBit j)
+  (hj3 : j = s.i + 2) :
+  (↑↑(inner_loop.next_coefficient s.i 2
+          (inner_loop.next_coefficient s.i 1
+              (inner_loop.next_coefficient s.i 0 (BitVec.setWidth 32 sample_bits)).1).1).2 : ZMod 3329) =
+    ∑ x : Fin s.η.val, ↑(Target.bytesToBits BVector)[2 * (s.i + 2) * ↑s.η + ↑x]!.toNat -
+      ∑ x : Fin s.η.val, ↑(Target.bytesToBits BVector)[2 * (s.i + 2) * ↑s.η + ↑s.η + ↑x]!.toNat := by
+  simp only [hη, Nat.mul_assoc 2 (s.i + 2) 2, Nat.mul_comm (s.i + 2) 2, ← Nat.mul_assoc 2 2 (s.i + 2),
+    Nat.reduceMul, Nat.mul_add 4, Nat.mul_comm 4 s.i, ← hs3, Fin.unfold2, Nat.mul_comm s.src_i 8]
+  conv in 8 * s.src_i + 8 + 0 => rw [(by omega : 8 * s.src_i + 8 + 0 = 8 * (s.src_i + 1) + 0)]
+  conv in 8 * s.src_i + 8 + 1 => rw [(by omega : 8 * s.src_i + 8 + 1 = 8 * (s.src_i + 1) + 1)]
+  conv in 8 * s.src_i + 8 + 2 + 0 => rw [(by omega : 8 * s.src_i + 8 + 2 + 0 = 8 * (s.src_i + 1) + 2)]
+  conv in 8 * s.src_i + 8 + 2 + 1 => rw [(by omega : 8 * s.src_i + 8 + 2 + 1 = 8 * (s.src_i + 1) + 3)]
+  rw [hBytesToBits (s.src_i + 1) (by scalar_tac) 0 (by omega),
+      hBytesToBits (s.src_i + 1) (by scalar_tac) 1 (by omega),
+      hBytesToBits (s.src_i + 1) (by scalar_tac) 2 (by omega),
+      hBytesToBits (s.src_i + 1) (by scalar_tac) 3 (by omega)]
+  unfold inner_loop.next_coefficient
+  simp only [BitVec.ofNat_eq_ofNat, ntt.Q.eq, UScalar.ofNat_val_eq, Nat.cast_ofNat, Nat.reduceAdd,
+    BitVec.toNat_add, BitVec.toNat_sub, Nat.reducePow, BitVec.toNat_ushiftRight, BitVec.toNat_and,
+    BitVec.toNat_setWidth, BitVec.toNat_ofNat, Nat.reduceMod, Nat.mod_add_mod, ← Nat.shiftRight_add]
+  olet hsample_bits_slice : sample_bits_slice := (sample_bits.toNat % 4294967296) >>> 8 &&& 15
+  olet hs_B_byte : s_B_byte := s.B[s.src_i + 1]!
+  replace hs_B_byte : sample_bits_slice = (s_B_byte &&& 5) + ((s_B_byte >>> 1) &&& 5) := by
+    rw [hsample_bits_slice, hsample_bits]
+    simp only [BitVec.toNat_add, BitVec.toNat_and, BitVec.toNat_ofNat,
+      BitVec.toNat_ushiftRight, Nat.mod_add_mod, BitVec.natCast_eq_ofNat, BitVec.ofNat_and,
+      Nat.cast_ofNat, BitVec.ofNat_eq_ofNat]
+    have sHB := s.hB
+    have hmin : min (s.B.size - s.src_i) 4 = 4 := by scalar_tac
+    simp only [List.slice_length, Array.length_toList, add_tsub_cancel_left]
+    olet hy : y := (BitVec.fromLEBytes (List.slice s.src_i (s.src_i + 4) s.B.toList)).toNat >>> 1
+    olet hx : x := (BitVec.fromLEBytes (List.slice s.src_i (s.src_i + 4) s.B.toList)).toNat
+    olet hx' : x' := (x &&& 1431655765 % 2 ^ (8 * min (s.B.size - s.src_i) 4))
+    olet hy' : y' := (y &&& 1431655765 % 2 ^ (8 * min (s.B.size - s.src_i) 4))
+    rw [Nat.mod_eq_of_lt] at hx' hy' <;> (try rw [hmin]; decide +native)
+    have hy'' : y' < 1431655765 + 1 := by
+      apply Nat.lt_succ_of_le
+      rw [hy']
+      exact Nat.and_le_right
+    have hx'' : x' < 1431655765 + 1 := by
+      apply Nat.lt_succ_of_le
+      rw [hx']
+      exact Nat.and_le_right
+    rw [Nat.mod_eq_of_lt, Nat.mod_eq_of_lt]
+    . rw [(by decide : 15#8 = 2#8^4 - 1#8), BitVec.and_two_pow_sub_one_eq_mod]
+      ext k hk1
+      by_cases hk2 : k < 4
+      . simp only [← BitVec.getElem!_eq_getElem, BitVec.getElem!_mod_pow2_eq _ _ _ hk2,
+          BitVec.getElem!_eq_testBit_toNat, BitVec.toNat_ofNat, Nat.reducePow, BitVec.toNat_add,
+          BitVec.toNat_and, Nat.reduceMod, BitVec.toNat_ushiftRight, Nat.mod_add_mod]
+        rw [testBitMod256 ((x' + y') >>> 8) k (by omega), Nat.mod_eq_of_lt]
+        . rw [hx', hy', hy, shiftDistribMask1431655765 (by omega) hk2, ← hy, ← hy', ← hx']
+          apply testBitOfAdd 4 _ _ k hk2
+          . intro i hi
+            simp only [hx', hx, Nat.testBit_shiftRight, Nat.testBit_and, ←
+              BitVec.getElem!_eq_testBit_toNat, BitVec.fromLEBytes_getElem!, Nat.ofNat_pos,
+              Nat.add_div_left, Nat.add_mod_left]
+            rw [List.getElem!_slice, hs_B_byte, Array.getElem!_toList]
+            . simp_scalar
+              congr 1
+              revert i
+              decide
+            . scalar_tac
+          . intro i hi
+            simp only [hy', hy, hx, Nat.testBit_and, Nat.testBit_shiftRight,
+              ← BitVec.getElem!_eq_testBit_toNat, BitVec.fromLEBytes_getElem!]
+            rw [(by omega : (1 + (8 + i)) / 8 = 1), (by omega : (1 + (8 + i)) % 8 = 1 + i),
+              List.getElem!_slice, hs_B_byte, Array.getElem!_toList]
+            . congr 1
+              revert i
+              decide
+            . scalar_tac
+        . have : BitVec.toNat s_B_byte &&& 5 ≤ 5 := Nat.and_le_right
+          have : (BitVec.toNat s_B_byte >>> 1) &&& 5 ≤ 5 := Nat.and_le_right
+          omega
+      . have : (s_B_byte &&& 5#8) + (s_B_byte >>> 1 &&& 5#8) < 2^4 := by
+          clear hs_B_byte hBytesToBits
+          revert s_B_byte
+          decide +native -- **TODO** Once `brute` supports unbounded UScalars, `brute` should be faster
+        rw [← BitVec.getElem!_eq_getElem, ← BitVec.getElem!_eq_getElem,
+          BitVec.getElem!_mod_pow2_false _ _ _ (by omega), BitVec.getElem!_eq_testBit_toNat,
+          ← Nat.mod_eq_of_lt this]
+        simp only [BitVec.toNat_add, BitVec.toNat_and, BitVec.toNat_ofNat, Nat.reducePow,
+          Nat.reduceMod, BitVec.toNat_ushiftRight, Nat.mod_add_mod, BitVec.ofNat_eq_ofNat,
+          BitVec.toNat_pow, Nat.reduceDvd, Nat.mod_mod_of_dvd, Bool.false_eq]
+        rw [(by decide : 16 = 2^4), Nat.testBit_mod_two_pow,
+          Bool.and_eq_false_eq_eq_false_or_eq_false]
+        left
+        simp only [decide_eq_false_iff_not, not_lt]
+        omega
+    . rw [hmin]; omega
+    . rw [hmin, Nat.mod_eq_of_lt] <;> omega
+  replace hsample_bits_slice : sample_bits_slice < 16 := by
+    rw [hsample_bits_slice]
+    exact Nat.lt_succ_of_le Nat.and_le_right
+  clear hBytesToBits
+  revert s_B_byte
+  revert sample_bits_slice
+  brute
+
+theorem Target2.samplePolyCBD.eta2_loop.spec.aux3 {s : samplePolyCBDState}
+  (BVector : Vector Byte (64 * ↑s.η))
+  (hBVector : BVector = ⟨s.B.take (64 * s.η), by have := s.hB; simp; omega⟩)
+  (hs1 : ∀ j < s.i, s.pe_dst[j]! = (Target.samplePolyCBD BVector)[j]!) (hs2 : ∀ j < 256, s.i ≤ j → s.pe_dst[j]! = 0)
+  (hs3 : s.src_i * 8 = s.i * 4) (hs4 : 8 ∣ s.i) (hs5 : 4 ∣ s.src_i) (hη : s.η.val = 2)
+  (hs6 : s.i < ↑key.MLWE_POLYNOMIAL_COEFFICIENTS) (j : ℕ) (hj1 : j < s.i + 8) (hj2 : ¬j < s.i)
+  (sample_bits : BitVec (8 * (List.slice s.src_i (s.src_i + 4) s.B.toList).length))
+  (hsample_bits :
+    sample_bits =
+      (BitVec.fromLEBytes (List.slice s.src_i (s.src_i + 4) s.B.toList) &&&
+          1431655765#(8 * (List.slice s.src_i (s.src_i + 4) s.B.toList).length)) +
+        (BitVec.fromLEBytes (List.slice s.src_i (s.src_i + 4) s.B.toList) >>> 1 &&&
+          1431655765#(8 * (List.slice s.src_i (s.src_i + 4) s.B.toList).length)))
+  (hBytesToBits : ∀ i < 64 * s.η.val, ∀ j < 8, (Target.bytesToBits BVector)[8 * i + j]! = s.B[i]!.testBit j)
+  (hj3 : j = s.i + 3) :
+  (↑↑(inner_loop.next_coefficient s.i 3
+          (inner_loop.next_coefficient s.i 2
+              (inner_loop.next_coefficient s.i 1
+                  (inner_loop.next_coefficient s.i 0 (BitVec.setWidth 32 sample_bits)).1).1).1).2 : ZMod 3329) =
+    ∑ x : Fin s.η.val, ↑(Target.bytesToBits BVector)[2 * (s.i + 3) * ↑s.η + ↑x]!.toNat -
+      ∑ x : Fin s.η.val, ↑(Target.bytesToBits BVector)[2 * (s.i + 3) * ↑s.η + ↑s.η + ↑x]!.toNat := by
+  simp only [hη, Nat.mul_assoc 2 (s.i + 3) 2, Nat.mul_comm (s.i + 3) 2, ← Nat.mul_assoc 2 2 (s.i + 3),
+    Nat.reduceMul, Nat.mul_add 4, Nat.mul_comm 4 s.i, ← hs3, Fin.unfold2, Nat.mul_comm s.src_i 8]
+  conv in 8 * s.src_i + 12 + 0 => rw [(by omega : 8 * s.src_i + 12 + 0 = 8 * (s.src_i + 1) + 4)]
+  conv in 8 * s.src_i + 12 + 1 => rw [(by omega : 8 * s.src_i + 12 + 1 = 8 * (s.src_i + 1) + 5)]
+  conv in 8 * s.src_i + 12 + 2 + 0 => rw [(by omega : 8 * s.src_i + 12 + 2 + 0 = 8 * (s.src_i + 1) + 6)]
+  conv in 8 * s.src_i + 12 + 2 + 1 => rw [(by omega : 8 * s.src_i + 12 + 2 + 1 = 8 * (s.src_i + 1) + 7)]
+  rw [hBytesToBits (s.src_i + 1) (by scalar_tac) 4 (by omega),
+      hBytesToBits (s.src_i + 1) (by scalar_tac) 5 (by omega),
+      hBytesToBits (s.src_i + 1) (by scalar_tac) 6 (by omega),
+      hBytesToBits (s.src_i + 1) (by scalar_tac) 7 (by omega)]
+  unfold inner_loop.next_coefficient
+  simp only [BitVec.ofNat_eq_ofNat, ntt.Q.eq, UScalar.ofNat_val_eq, Nat.cast_ofNat, Nat.reduceAdd,
+    BitVec.toNat_add, BitVec.toNat_sub, Nat.reducePow, BitVec.toNat_ushiftRight, BitVec.toNat_and,
+    BitVec.toNat_setWidth, BitVec.toNat_ofNat, Nat.reduceMod, Nat.mod_add_mod, ← Nat.shiftRight_add]
+  olet hsample_bits_slice : sample_bits_slice := (sample_bits.toNat % 4294967296) >>> 12 &&& 15
+  olet hs_B_byte : s_B_byte := s.B[s.src_i + 1]!
+  replace hs_B_byte : sample_bits_slice = ((s_B_byte >>> 4) &&& 5) + ((s_B_byte >>> 5) &&& 5) := by
+    rw [hsample_bits_slice, hsample_bits]
+    simp only [BitVec.toNat_add, BitVec.toNat_and, BitVec.toNat_ofNat,
+      BitVec.toNat_ushiftRight, Nat.mod_add_mod, BitVec.natCast_eq_ofNat, BitVec.ofNat_and,
+      Nat.cast_ofNat, BitVec.ofNat_eq_ofNat]
+    have sHB := s.hB
+    have hmin : min (s.B.size - s.src_i) 4 = 4 := by scalar_tac
+    simp only [List.slice_length, Array.length_toList, add_tsub_cancel_left]
+    olet hy : y := (BitVec.fromLEBytes (List.slice s.src_i (s.src_i + 4) s.B.toList)).toNat >>> 1
+    olet hx : x := (BitVec.fromLEBytes (List.slice s.src_i (s.src_i + 4) s.B.toList)).toNat
+    olet hx' : x' := (x &&& 1431655765 % 2 ^ (8 * min (s.B.size - s.src_i) 4))
+    olet hy' : y' := (y &&& 1431655765 % 2 ^ (8 * min (s.B.size - s.src_i) 4))
+    rw [Nat.mod_eq_of_lt] at hx' hy' <;> (try rw [hmin]; decide +native)
+    have hy'' : y' < 1431655765 + 1 := by
+      apply Nat.lt_succ_of_le
+      rw [hy']
+      exact Nat.and_le_right
+    have hx'' : x' < 1431655765 + 1 := by
+      apply Nat.lt_succ_of_le
+      rw [hx']
+      exact Nat.and_le_right
+    rw [Nat.mod_eq_of_lt, Nat.mod_eq_of_lt]
+    . rw [(by decide : 15#8 = 2#8^4 - 1#8), BitVec.and_two_pow_sub_one_eq_mod]
+      ext k hk1
+      by_cases hk2 : k < 4
+      . simp only [← BitVec.getElem!_eq_getElem, BitVec.getElem!_mod_pow2_eq _ _ _ hk2,
+          BitVec.getElem!_eq_testBit_toNat, BitVec.toNat_ofNat, Nat.reducePow, BitVec.toNat_add,
+          BitVec.toNat_and, Nat.reduceMod, BitVec.toNat_ushiftRight, Nat.mod_add_mod]
+        rw [testBitMod256 ((x' + y') >>> 12) k (by omega), Nat.mod_eq_of_lt]
+        . rw [hx', hy', hy, shiftDistribMask1431655765 (by omega) hk2, ← hy, ← hy', ← hx']
+          apply testBitOfAdd 4 _ _ k hk2
+          . intro i hi
+            simp only [hx', hx, Nat.testBit_shiftRight, Nat.testBit_and,
+              ← BitVec.getElem!_eq_testBit_toNat, BitVec.fromLEBytes_getElem!]
+            rw [List.getElem!_slice, hs_B_byte, Array.getElem!_toList]
+            . rw [(by omega : (12 + i) / 8 = 1), (by omega : (12 + i) % 8 = 4 + i)]
+              simp_scalar
+              congr 1
+              revert i
+              decide
+            . scalar_tac
+          . intro i hi
+            simp only [hy', hy, hx, Nat.testBit_and, Nat.testBit_shiftRight,
+              ← BitVec.getElem!_eq_testBit_toNat, BitVec.fromLEBytes_getElem!]
+            by_cases hi2 : i < 3
+            . rw [(by omega : (1 + (12 + i)) / 8 = 1), (by omega : (1 + (12 + i)) % 8 = 5 + i),
+                List.getElem!_slice, hs_B_byte, Array.getElem!_toList]
+              . congr 1
+                revert i
+                decide
+              . scalar_tac
+            . have h1 : Nat.testBit 1431655765 (12 + i) = false := by revert i; decide
+              have h2 : Nat.testBit 5 i = false := by revert i; decide
+              simp only [h1, Bool.and_false, h2]
+        . have : (BitVec.toNat s_B_byte >>> 4) &&& 5 ≤ 5 := Nat.and_le_right
+          have : (BitVec.toNat s_B_byte >>> 5) &&& 5 ≤ 5 := Nat.and_le_right
+          omega
+      . have : (s_B_byte >>> 4 &&& 5#8) + (s_B_byte >>> 5 &&& 5#8) < 2^4 := by
+          clear hs_B_byte hBytesToBits
+          revert s_B_byte
+          decide +native -- **TODO** Once `brute` supports unbounded UScalars, `brute` should be faster
+        rw [← BitVec.getElem!_eq_getElem, ← BitVec.getElem!_eq_getElem,
+          BitVec.getElem!_mod_pow2_false _ _ _ (by omega), BitVec.getElem!_eq_testBit_toNat,
+          ← Nat.mod_eq_of_lt this]
+        simp only [BitVec.toNat_add, BitVec.toNat_and, BitVec.toNat_ofNat, Nat.reducePow,
+          Nat.reduceMod, BitVec.toNat_ushiftRight, Nat.mod_add_mod, BitVec.ofNat_eq_ofNat,
+          BitVec.toNat_pow, Nat.reduceDvd, Nat.mod_mod_of_dvd, Bool.false_eq]
+        rw [(by decide : 16 = 2^4), Nat.testBit_mod_two_pow,
+          Bool.and_eq_false_eq_eq_false_or_eq_false]
+        left
+        simp only [decide_eq_false_iff_not, not_lt]
+        omega
+    . rw [hmin]; omega
+    . rw [hmin, Nat.mod_eq_of_lt] <;> omega
+  replace hsample_bits_slice : sample_bits_slice < 16 := by
+    rw [hsample_bits_slice]
+    exact Nat.lt_succ_of_le Nat.and_le_right
+  clear hBytesToBits
+  revert s_B_byte
+  revert sample_bits_slice
+  brute
+
+theorem Target2.samplePolyCBD.eta2_loop.spec.aux4 {s : samplePolyCBDState}
+  (BVector : Vector Byte (64 * ↑s.η))
+  (hBVector : BVector = ⟨s.B.take (64 * s.η), by have := s.hB; simp; omega⟩)
+  (hs1 : ∀ j < s.i, s.pe_dst[j]! = (Target.samplePolyCBD BVector)[j]!) (hs2 : ∀ j < 256, s.i ≤ j → s.pe_dst[j]! = 0)
+  (hs3 : s.src_i * 8 = s.i * 4) (hs4 : 8 ∣ s.i) (hs5 : 4 ∣ s.src_i) (hη : s.η.val = 2)
+  (hs6 : s.i < ↑key.MLWE_POLYNOMIAL_COEFFICIENTS) (j : ℕ) (hj1 : j < s.i + 8) (hj2 : ¬j < s.i)
+  (sample_bits : BitVec (8 * (List.slice s.src_i (s.src_i + 4) s.B.toList).length))
+  (hsample_bits :
+    sample_bits =
+      (BitVec.fromLEBytes (List.slice s.src_i (s.src_i + 4) s.B.toList) &&&
+          1431655765#(8 * (List.slice s.src_i (s.src_i + 4) s.B.toList).length)) +
+        (BitVec.fromLEBytes (List.slice s.src_i (s.src_i + 4) s.B.toList) >>> 1 &&&
+          1431655765#(8 * (List.slice s.src_i (s.src_i + 4) s.B.toList).length)))
+  (hBytesToBits : ∀ i < 64 * s.η.val, ∀ j < 8, (Target.bytesToBits BVector)[8 * i + j]! = s.B[i]!.testBit j)
+  (hj3 : j = s.i + 4) :
+  (↑↑(inner_loop.next_coefficient s.i 4
+          (inner_loop.next_coefficient s.i 3
+              (inner_loop.next_coefficient s.i 2
+                  (inner_loop.next_coefficient s.i 1
+                      (inner_loop.next_coefficient s.i 0 (BitVec.setWidth 32 sample_bits)).1).1).1).1).2 : ZMod 3329) =
+    ∑ x : Fin s.η.val, ↑(Target.bytesToBits BVector)[2 * (s.i + 4) * ↑s.η + ↑x]!.toNat -
+      ∑ x : Fin s.η.val, ↑(Target.bytesToBits BVector)[2 * (s.i + 4) * ↑s.η + ↑s.η + ↑x]!.toNat := by
+  simp only [hη, Nat.mul_assoc 2 (s.i + 4) 2, Nat.mul_comm (s.i + 4) 2, ← Nat.mul_assoc 2 2 (s.i + 4),
+    Nat.reduceMul, Nat.mul_add 4, Nat.mul_comm 4 s.i, ← hs3, Fin.unfold2, Nat.mul_comm s.src_i 8]
+  conv in 8 * s.src_i + 16 + 0 => rw [(by omega : 8 * s.src_i + 16 + 0 = 8 * (s.src_i + 2) + 0)]
+  conv in 8 * s.src_i + 16 + 1 => rw [(by omega : 8 * s.src_i + 16 + 1 = 8 * (s.src_i + 2) + 1)]
+  conv in 8 * s.src_i + 16 + 2 + 0 => rw [(by omega : 8 * s.src_i + 16 + 2 + 0 = 8 * (s.src_i + 2) + 2)]
+  conv in 8 * s.src_i + 16 + 2 + 1 => rw [(by omega : 8 * s.src_i + 16 + 2 + 1 = 8 * (s.src_i + 2) + 3)]
+  rw [hBytesToBits (s.src_i + 2) (by scalar_tac) 0 (by omega),
+      hBytesToBits (s.src_i + 2) (by scalar_tac) 1 (by omega),
+      hBytesToBits (s.src_i + 2) (by scalar_tac) 2 (by omega),
+      hBytesToBits (s.src_i + 2) (by scalar_tac) 3 (by omega)]
+  unfold inner_loop.next_coefficient
+  simp only [BitVec.ofNat_eq_ofNat, ntt.Q.eq, UScalar.ofNat_val_eq, Nat.cast_ofNat, Nat.reduceAdd,
+    BitVec.toNat_add, BitVec.toNat_sub, Nat.reducePow, BitVec.toNat_ushiftRight, BitVec.toNat_and,
+    BitVec.toNat_setWidth, BitVec.toNat_ofNat, Nat.reduceMod, Nat.mod_add_mod, ← Nat.shiftRight_add]
+  olet hsample_bits_slice : sample_bits_slice := (sample_bits.toNat % 4294967296) >>> 16 &&& 15
+  olet hs_B_byte : s_B_byte := s.B[s.src_i + 2]!
+  replace hs_B_byte : sample_bits_slice = (s_B_byte &&& 5) + ((s_B_byte >>> 1) &&& 5) := by
+    rw [hsample_bits_slice, hsample_bits]
+    simp only [BitVec.toNat_add, BitVec.toNat_and, BitVec.toNat_ofNat,
+      BitVec.toNat_ushiftRight, Nat.mod_add_mod, BitVec.natCast_eq_ofNat, BitVec.ofNat_and,
+      Nat.cast_ofNat, BitVec.ofNat_eq_ofNat]
+    have sHB := s.hB
+    have hmin : min (s.B.size - s.src_i) 4 = 4 := by scalar_tac
+    simp only [List.slice_length, Array.length_toList, add_tsub_cancel_left]
+    olet hy : y := (BitVec.fromLEBytes (List.slice s.src_i (s.src_i + 4) s.B.toList)).toNat >>> 1
+    olet hx : x := (BitVec.fromLEBytes (List.slice s.src_i (s.src_i + 4) s.B.toList)).toNat
+    olet hx' : x' := (x &&& 1431655765 % 2 ^ (8 * min (s.B.size - s.src_i) 4))
+    olet hy' : y' := (y &&& 1431655765 % 2 ^ (8 * min (s.B.size - s.src_i) 4))
+    rw [Nat.mod_eq_of_lt] at hx' hy' <;> (try rw [hmin]; decide +native)
+    have hy'' : y' < 1431655765 + 1 := by
+      apply Nat.lt_succ_of_le
+      rw [hy']
+      exact Nat.and_le_right
+    have hx'' : x' < 1431655765 + 1 := by
+      apply Nat.lt_succ_of_le
+      rw [hx']
+      exact Nat.and_le_right
+    rw [Nat.mod_eq_of_lt, Nat.mod_eq_of_lt]
+    . rw [(by decide : 15#8 = 2#8^4 - 1#8), BitVec.and_two_pow_sub_one_eq_mod]
+      ext k hk1
+      by_cases hk2 : k < 4
+      . simp only [← BitVec.getElem!_eq_getElem, BitVec.getElem!_mod_pow2_eq _ _ _ hk2,
+          BitVec.getElem!_eq_testBit_toNat, BitVec.toNat_ofNat, Nat.reducePow, BitVec.toNat_add,
+          BitVec.toNat_and, Nat.reduceMod, BitVec.toNat_ushiftRight, Nat.mod_add_mod]
+        rw [testBitMod256 ((x' + y') >>> 16) k (by omega), Nat.mod_eq_of_lt]
+        . rw [hx', hy', hy, shiftDistribMask1431655765 (by omega) hk2, ← hy, ← hy', ← hx']
+          apply testBitOfAdd 4 _ _ k hk2
+          . intro i hi
+            simp only [hx', hx, Nat.testBit_shiftRight, Nat.testBit_and, ←
+              BitVec.getElem!_eq_testBit_toNat, BitVec.fromLEBytes_getElem!, Nat.ofNat_pos,
+              Nat.add_div_left, Nat.add_mod_left]
+            rw [List.getElem!_slice, hs_B_byte, Array.getElem!_toList]
+            . rw [(by omega : (16 + i) / 8 = 2), (by omega : (16 + i) % 8 = i)]
+              simp_scalar
+              congr 1
+              revert i
+              decide
+            . scalar_tac
+          . intro i hi
+            simp only [hy', hy, hx, Nat.testBit_and, Nat.testBit_shiftRight,
+              ← BitVec.getElem!_eq_testBit_toNat, BitVec.fromLEBytes_getElem!]
+            rw [(by omega : (1 + (16 + i)) / 8 = 2), (by omega : (1 + (16 + i)) % 8 = 1 + i),
+              List.getElem!_slice, hs_B_byte, Array.getElem!_toList]
+            . congr 1
+              revert i
+              decide
+            . scalar_tac
+        . have : BitVec.toNat s_B_byte &&& 5 ≤ 5 := Nat.and_le_right
+          have : (BitVec.toNat s_B_byte >>> 1) &&& 5 ≤ 5 := Nat.and_le_right
+          omega
+      . have : (s_B_byte &&& 5#8) + (s_B_byte >>> 1 &&& 5#8) < 2^4 := by
+          clear hs_B_byte hBytesToBits
+          revert s_B_byte
+          decide +native -- **TODO** Once `brute` supports unbounded UScalars, `brute` should be faster
+        rw [← BitVec.getElem!_eq_getElem, ← BitVec.getElem!_eq_getElem,
+          BitVec.getElem!_mod_pow2_false _ _ _ (by omega), BitVec.getElem!_eq_testBit_toNat,
+          ← Nat.mod_eq_of_lt this]
+        simp only [BitVec.toNat_add, BitVec.toNat_and, BitVec.toNat_ofNat, Nat.reducePow,
+          Nat.reduceMod, BitVec.toNat_ushiftRight, Nat.mod_add_mod, BitVec.ofNat_eq_ofNat,
+          BitVec.toNat_pow, Nat.reduceDvd, Nat.mod_mod_of_dvd, Bool.false_eq]
+        rw [(by decide : 16 = 2^4), Nat.testBit_mod_two_pow,
+          Bool.and_eq_false_eq_eq_false_or_eq_false]
+        left
+        simp only [decide_eq_false_iff_not, not_lt]
+        omega
+    . rw [hmin]; omega
+    . rw [hmin, Nat.mod_eq_of_lt] <;> omega
+  replace hsample_bits_slice : sample_bits_slice < 16 := by
+    rw [hsample_bits_slice]
+    exact Nat.lt_succ_of_le Nat.and_le_right
+  clear hBytesToBits
+  revert s_B_byte
+  revert sample_bits_slice
+  brute
+
+theorem Target2.samplePolyCBD.eta2_loop.spec.aux5 {s : samplePolyCBDState}
+  (BVector : Vector Byte (64 * ↑s.η))
+  (hBVector : BVector = ⟨s.B.take (64 * s.η), by have := s.hB; simp; omega⟩)
+  (hs1 : ∀ j < s.i, s.pe_dst[j]! = (Target.samplePolyCBD BVector)[j]!) (hs2 : ∀ j < 256, s.i ≤ j → s.pe_dst[j]! = 0)
+  (hs3 : s.src_i * 8 = s.i * 4) (hs4 : 8 ∣ s.i) (hs5 : 4 ∣ s.src_i) (hη : s.η.val = 2)
+  (hs6 : s.i < ↑key.MLWE_POLYNOMIAL_COEFFICIENTS) (j : ℕ) (hj1 : j < s.i + 8) (hj2 : ¬j < s.i)
+  (sample_bits : BitVec (8 * (List.slice s.src_i (s.src_i + 4) s.B.toList).length))
+  (hsample_bits :
+    sample_bits =
+      (BitVec.fromLEBytes (List.slice s.src_i (s.src_i + 4) s.B.toList) &&&
+          1431655765#(8 * (List.slice s.src_i (s.src_i + 4) s.B.toList).length)) +
+        (BitVec.fromLEBytes (List.slice s.src_i (s.src_i + 4) s.B.toList) >>> 1 &&&
+          1431655765#(8 * (List.slice s.src_i (s.src_i + 4) s.B.toList).length)))
+  (hBytesToBits : ∀ i < 64 * s.η.val, ∀ j < 8, (Target.bytesToBits BVector)[8 * i + j]! = s.B[i]!.testBit j)
+  (hj3 : j = s.i + 5) :
+  (↑↑(inner_loop.next_coefficient s.i 5
+      (inner_loop.next_coefficient s.i 4
+      (inner_loop.next_coefficient s.i 3
+      (inner_loop.next_coefficient s.i 2
+      (inner_loop.next_coefficient s.i 1
+      (inner_loop.next_coefficient s.i 0 (BitVec.setWidth 32 sample_bits)).1).1).1).1).1).2 : ZMod 3329) =
+    ∑ x : Fin s.η.val, ↑(Target.bytesToBits BVector)[2 * (s.i + 5) * ↑s.η + ↑x]!.toNat -
+      ∑ x : Fin s.η.val, ↑(Target.bytesToBits BVector)[2 * (s.i + 5) * ↑s.η + ↑s.η + ↑x]!.toNat := by
+  simp only [hη, Nat.mul_assoc 2 (s.i + 5) 2, Nat.mul_comm (s.i + 5) 2, ← Nat.mul_assoc 2 2 (s.i + 5),
+    Nat.reduceMul, Nat.mul_add 4, Nat.mul_comm 4 s.i, ← hs3, Fin.unfold2, Nat.mul_comm s.src_i 8]
+  conv in 8 * s.src_i + 20 + 0 => rw [(by omega : 8 * s.src_i + 20 + 0 = 8 * (s.src_i + 2) + 4)]
+  conv in 8 * s.src_i + 20 + 1 => rw [(by omega : 8 * s.src_i + 20 + 1 = 8 * (s.src_i + 2) + 5)]
+  conv in 8 * s.src_i + 20 + 2 + 0 => rw [(by omega : 8 * s.src_i + 20 + 2 + 0 = 8 * (s.src_i + 2) + 6)]
+  conv in 8 * s.src_i + 20 + 2 + 1 => rw [(by omega : 8 * s.src_i + 20 + 2 + 1 = 8 * (s.src_i + 2) + 7)]
+  rw [hBytesToBits (s.src_i + 2) (by scalar_tac) 4 (by omega),
+      hBytesToBits (s.src_i + 2) (by scalar_tac) 5 (by omega),
+      hBytesToBits (s.src_i + 2) (by scalar_tac) 6 (by omega),
+      hBytesToBits (s.src_i + 2) (by scalar_tac) 7 (by omega)]
+  unfold inner_loop.next_coefficient
+  simp only [BitVec.ofNat_eq_ofNat, ntt.Q.eq, UScalar.ofNat_val_eq, Nat.cast_ofNat, Nat.reduceAdd,
+    BitVec.toNat_add, BitVec.toNat_sub, Nat.reducePow, BitVec.toNat_ushiftRight, BitVec.toNat_and,
+    BitVec.toNat_setWidth, BitVec.toNat_ofNat, Nat.reduceMod, Nat.mod_add_mod, ← Nat.shiftRight_add]
+  olet hsample_bits_slice : sample_bits_slice := (sample_bits.toNat % 4294967296) >>> 20 &&& 15
+  olet hs_B_byte : s_B_byte := s.B[s.src_i + 2]!
+  replace hs_B_byte : sample_bits_slice = ((s_B_byte >>> 4) &&& 5) + ((s_B_byte >>> 5) &&& 5) := by
+    rw [hsample_bits_slice, hsample_bits]
+    simp only [BitVec.toNat_add, BitVec.toNat_and, BitVec.toNat_ofNat,
+      BitVec.toNat_ushiftRight, Nat.mod_add_mod, BitVec.natCast_eq_ofNat, BitVec.ofNat_and,
+      Nat.cast_ofNat, BitVec.ofNat_eq_ofNat]
+    have sHB := s.hB
+    have hmin : min (s.B.size - s.src_i) 4 = 4 := by scalar_tac
+    simp only [List.slice_length, Array.length_toList, add_tsub_cancel_left]
+    olet hy : y := (BitVec.fromLEBytes (List.slice s.src_i (s.src_i + 4) s.B.toList)).toNat >>> 1
+    olet hx : x := (BitVec.fromLEBytes (List.slice s.src_i (s.src_i + 4) s.B.toList)).toNat
+    olet hx' : x' := (x &&& 1431655765 % 2 ^ (8 * min (s.B.size - s.src_i) 4))
+    olet hy' : y' := (y &&& 1431655765 % 2 ^ (8 * min (s.B.size - s.src_i) 4))
+    rw [Nat.mod_eq_of_lt] at hx' hy' <;> (try rw [hmin]; decide +native)
+    have hy'' : y' < 1431655765 + 1 := by
+      apply Nat.lt_succ_of_le
+      rw [hy']
+      exact Nat.and_le_right
+    have hx'' : x' < 1431655765 + 1 := by
+      apply Nat.lt_succ_of_le
+      rw [hx']
+      exact Nat.and_le_right
+    rw [Nat.mod_eq_of_lt, Nat.mod_eq_of_lt]
+    . rw [(by decide : 15#8 = 2#8^4 - 1#8), BitVec.and_two_pow_sub_one_eq_mod]
+      ext k hk1
+      by_cases hk2 : k < 4
+      . simp only [← BitVec.getElem!_eq_getElem, BitVec.getElem!_mod_pow2_eq _ _ _ hk2,
+          BitVec.getElem!_eq_testBit_toNat, BitVec.toNat_ofNat, Nat.reducePow, BitVec.toNat_add,
+          BitVec.toNat_and, Nat.reduceMod, BitVec.toNat_ushiftRight, Nat.mod_add_mod]
+        rw [testBitMod256 ((x' + y') >>> 20) k (by omega), Nat.mod_eq_of_lt]
+        . rw [hx', hy', hy, shiftDistribMask1431655765 (by omega) hk2, ← hy, ← hy', ← hx']
+          apply testBitOfAdd 4 _ _ k hk2
+          . intro i hi
+            simp only [hx', hx, Nat.testBit_shiftRight, Nat.testBit_and,
+              ← BitVec.getElem!_eq_testBit_toNat, BitVec.fromLEBytes_getElem!]
+            rw [List.getElem!_slice, hs_B_byte, Array.getElem!_toList]
+            . rw [(by omega : (20 + i) / 8 = 2), (by omega : (20 + i) % 8 = 4 + i)]
+              simp_scalar
+              congr 1
+              revert i
+              decide
+            . scalar_tac
+          . intro i hi
+            simp only [hy', hy, hx, Nat.testBit_and, Nat.testBit_shiftRight,
+              ← BitVec.getElem!_eq_testBit_toNat, BitVec.fromLEBytes_getElem!]
+            by_cases hi2 : i < 3
+            . rw [(by omega : (1 + (20 + i)) / 8 = 2), (by omega : (1 + (20 + i)) % 8 = 5 + i),
+                List.getElem!_slice, hs_B_byte, Array.getElem!_toList]
+              . congr 1
+                revert i
+                decide
+              . scalar_tac
+            . have h1 : Nat.testBit 1431655765 (20 + i) = false := by revert i; decide
+              have h2 : Nat.testBit 5 i = false := by revert i; decide
+              simp only [h1, Bool.and_false, h2]
+        . have : (BitVec.toNat s_B_byte >>> 4) &&& 5 ≤ 5 := Nat.and_le_right
+          have : (BitVec.toNat s_B_byte >>> 5) &&& 5 ≤ 5 := Nat.and_le_right
+          omega
+      . have : (s_B_byte >>> 4 &&& 5#8) + (s_B_byte >>> 5 &&& 5#8) < 2^4 := by
+          clear hs_B_byte hBytesToBits
+          revert s_B_byte
+          decide +native -- **TODO** Once `brute` supports unbounded UScalars, `brute` should be faster
+        rw [← BitVec.getElem!_eq_getElem, ← BitVec.getElem!_eq_getElem,
+          BitVec.getElem!_mod_pow2_false _ _ _ (by omega), BitVec.getElem!_eq_testBit_toNat,
+          ← Nat.mod_eq_of_lt this]
+        simp only [BitVec.toNat_add, BitVec.toNat_and, BitVec.toNat_ofNat, Nat.reducePow,
+          Nat.reduceMod, BitVec.toNat_ushiftRight, Nat.mod_add_mod, BitVec.ofNat_eq_ofNat,
+          BitVec.toNat_pow, Nat.reduceDvd, Nat.mod_mod_of_dvd, Bool.false_eq]
+        rw [(by decide : 16 = 2^4), Nat.testBit_mod_two_pow,
+          Bool.and_eq_false_eq_eq_false_or_eq_false]
+        left
+        simp only [decide_eq_false_iff_not, not_lt]
+        omega
+    . rw [hmin]; omega
+    . rw [hmin, Nat.mod_eq_of_lt] <;> omega
+  replace hsample_bits_slice : sample_bits_slice < 16 := by
+    rw [hsample_bits_slice]
+    exact Nat.lt_succ_of_le Nat.and_le_right
+  clear hBytesToBits
+  revert s_B_byte
+  revert sample_bits_slice
+  brute
+
+theorem Target2.samplePolyCBD.eta2_loop.spec.aux6 {s : samplePolyCBDState}
+  (BVector : Vector Byte (64 * ↑s.η))
+  (hBVector : BVector = ⟨s.B.take (64 * s.η), by have := s.hB; simp; omega⟩)
+  (hs1 : ∀ j < s.i, s.pe_dst[j]! = (Target.samplePolyCBD BVector)[j]!) (hs2 : ∀ j < 256, s.i ≤ j → s.pe_dst[j]! = 0)
+  (hs3 : s.src_i * 8 = s.i * 4) (hs4 : 8 ∣ s.i) (hs5 : 4 ∣ s.src_i) (hη : s.η.val = 2)
+  (hs6 : s.i < ↑key.MLWE_POLYNOMIAL_COEFFICIENTS) (j : ℕ) (hj1 : j < s.i + 8) (hj2 : ¬j < s.i)
+  (sample_bits : BitVec (8 * (List.slice s.src_i (s.src_i + 4) s.B.toList).length))
+  (hsample_bits :
+    sample_bits =
+      (BitVec.fromLEBytes (List.slice s.src_i (s.src_i + 4) s.B.toList) &&&
+          1431655765#(8 * (List.slice s.src_i (s.src_i + 4) s.B.toList).length)) +
+        (BitVec.fromLEBytes (List.slice s.src_i (s.src_i + 4) s.B.toList) >>> 1 &&&
+          1431655765#(8 * (List.slice s.src_i (s.src_i + 4) s.B.toList).length)))
+  (hBytesToBits : ∀ i < 64 * s.η.val, ∀ j < 8, (Target.bytesToBits BVector)[8 * i + j]! = s.B[i]!.testBit j)
+  (hj3 : j = s.i + 6) :
+  (↑↑(inner_loop.next_coefficient s.i 6
+      (inner_loop.next_coefficient s.i 5
+      (inner_loop.next_coefficient s.i 4
+      (inner_loop.next_coefficient s.i 3
+      (inner_loop.next_coefficient s.i 2
+      (inner_loop.next_coefficient s.i 1
+      (inner_loop.next_coefficient s.i 0 (BitVec.setWidth 32 sample_bits)).1).1).1).1).1).1).2 : ZMod 3329) =
+    ∑ x : Fin s.η.val, ↑(Target.bytesToBits BVector)[2 * (s.i + 6) * ↑s.η + ↑x]!.toNat -
+      ∑ x : Fin s.η.val, ↑(Target.bytesToBits BVector)[2 * (s.i + 6) * ↑s.η + ↑s.η + ↑x]!.toNat := by
+  simp only [hη, Nat.mul_assoc 2 (s.i + 6) 2, Nat.mul_comm (s.i + 6) 2, ← Nat.mul_assoc 2 2 (s.i + 6),
+    Nat.reduceMul, Nat.mul_add 4, Nat.mul_comm 4 s.i, ← hs3, Fin.unfold2, Nat.mul_comm s.src_i 8]
+  conv in 8 * s.src_i + 24 + 0 => rw [(by omega : 8 * s.src_i + 24 + 0 = 8 * (s.src_i + 3) + 0)]
+  conv in 8 * s.src_i + 24 + 1 => rw [(by omega : 8 * s.src_i + 24 + 1 = 8 * (s.src_i + 3) + 1)]
+  conv in 8 * s.src_i + 24 + 2 + 0 => rw [(by omega : 8 * s.src_i + 24 + 2 + 0 = 8 * (s.src_i + 3) + 2)]
+  conv in 8 * s.src_i + 24 + 2 + 1 => rw [(by omega : 8 * s.src_i + 24 + 2 + 1 = 8 * (s.src_i + 3) + 3)]
+  rw [hBytesToBits (s.src_i + 3) (by scalar_tac) 0 (by omega),
+      hBytesToBits (s.src_i + 3) (by scalar_tac) 1 (by omega),
+      hBytesToBits (s.src_i + 3) (by scalar_tac) 2 (by omega),
+      hBytesToBits (s.src_i + 3) (by scalar_tac) 3 (by omega)]
+  unfold inner_loop.next_coefficient
+  simp only [BitVec.ofNat_eq_ofNat, ntt.Q.eq, UScalar.ofNat_val_eq, Nat.cast_ofNat, Nat.reduceAdd,
+    BitVec.toNat_add, BitVec.toNat_sub, Nat.reducePow, BitVec.toNat_ushiftRight, BitVec.toNat_and,
+    BitVec.toNat_setWidth, BitVec.toNat_ofNat, Nat.reduceMod, Nat.mod_add_mod, ← Nat.shiftRight_add]
+  olet hsample_bits_slice : sample_bits_slice := (sample_bits.toNat % 4294967296) >>> 24 &&& 15
+  olet hs_B_byte : s_B_byte := s.B[s.src_i + 3]!
+  replace hs_B_byte : sample_bits_slice = (s_B_byte &&& 5) + ((s_B_byte >>> 1) &&& 5) := by
+    rw [hsample_bits_slice, hsample_bits]
+    simp only [BitVec.toNat_add, BitVec.toNat_and, BitVec.toNat_ofNat,
+      BitVec.toNat_ushiftRight, Nat.mod_add_mod, BitVec.natCast_eq_ofNat, BitVec.ofNat_and,
+      Nat.cast_ofNat, BitVec.ofNat_eq_ofNat]
+    have sHB := s.hB
+    have hmin : min (s.B.size - s.src_i) 4 = 4 := by scalar_tac
+    simp only [List.slice_length, Array.length_toList, add_tsub_cancel_left]
+    olet hy : y := (BitVec.fromLEBytes (List.slice s.src_i (s.src_i + 4) s.B.toList)).toNat >>> 1
+    olet hx : x := (BitVec.fromLEBytes (List.slice s.src_i (s.src_i + 4) s.B.toList)).toNat
+    olet hx' : x' := (x &&& 1431655765 % 2 ^ (8 * min (s.B.size - s.src_i) 4))
+    olet hy' : y' := (y &&& 1431655765 % 2 ^ (8 * min (s.B.size - s.src_i) 4))
+    rw [Nat.mod_eq_of_lt] at hx' hy' <;> (try rw [hmin]; decide +native)
+    have hy'' : y' < 1431655765 + 1 := by
+      apply Nat.lt_succ_of_le
+      rw [hy']
+      exact Nat.and_le_right
+    have hx'' : x' < 1431655765 + 1 := by
+      apply Nat.lt_succ_of_le
+      rw [hx']
+      exact Nat.and_le_right
+    rw [Nat.mod_eq_of_lt, Nat.mod_eq_of_lt]
+    . rw [(by decide : 15#8 = 2#8^4 - 1#8), BitVec.and_two_pow_sub_one_eq_mod]
+      ext k hk1
+      by_cases hk2 : k < 4
+      . simp only [← BitVec.getElem!_eq_getElem, BitVec.getElem!_mod_pow2_eq _ _ _ hk2,
+          BitVec.getElem!_eq_testBit_toNat, BitVec.toNat_ofNat, Nat.reducePow, BitVec.toNat_add,
+          BitVec.toNat_and, Nat.reduceMod, BitVec.toNat_ushiftRight, Nat.mod_add_mod]
+        rw [testBitMod256 ((x' + y') >>> 24) k (by omega), Nat.mod_eq_of_lt]
+        . rw [hx', hy', hy, shiftDistribMask1431655765 (by omega) hk2, ← hy, ← hy', ← hx']
+          apply testBitOfAdd 4 _ _ k hk2
+          . intro i hi
+            simp only [hx', hx, Nat.testBit_shiftRight, Nat.testBit_and, ←
+              BitVec.getElem!_eq_testBit_toNat, BitVec.fromLEBytes_getElem!, Nat.ofNat_pos,
+              Nat.add_div_left, Nat.add_mod_left]
+            rw [List.getElem!_slice, hs_B_byte, Array.getElem!_toList]
+            . rw [(by omega : (24 + i) / 8 = 3), (by omega : (24 + i) % 8 = i)]
+              simp_scalar
+              congr 1
+              revert i
+              decide
+            . scalar_tac
+          . intro i hi
+            simp only [hy', hy, hx, Nat.testBit_and, Nat.testBit_shiftRight,
+              ← BitVec.getElem!_eq_testBit_toNat, BitVec.fromLEBytes_getElem!]
+            rw [(by omega : (1 + (24 + i)) / 8 = 3), (by omega : (1 + (24 + i)) % 8 = 1 + i),
+              List.getElem!_slice, hs_B_byte, Array.getElem!_toList]
+            . congr 1
+              revert i
+              decide
+            . scalar_tac
+        . have : BitVec.toNat s_B_byte &&& 5 ≤ 5 := Nat.and_le_right
+          have : (BitVec.toNat s_B_byte >>> 1) &&& 5 ≤ 5 := Nat.and_le_right
+          omega
+      . have : (s_B_byte &&& 5#8) + (s_B_byte >>> 1 &&& 5#8) < 2^4 := by
+          clear hs_B_byte hBytesToBits
+          revert s_B_byte
+          decide +native -- **TODO** Once `brute` supports unbounded UScalars, `brute` should be faster
+        rw [← BitVec.getElem!_eq_getElem, ← BitVec.getElem!_eq_getElem,
+          BitVec.getElem!_mod_pow2_false _ _ _ (by omega), BitVec.getElem!_eq_testBit_toNat,
+          ← Nat.mod_eq_of_lt this]
+        simp only [BitVec.toNat_add, BitVec.toNat_and, BitVec.toNat_ofNat, Nat.reducePow,
+          Nat.reduceMod, BitVec.toNat_ushiftRight, Nat.mod_add_mod, BitVec.ofNat_eq_ofNat,
+          BitVec.toNat_pow, Nat.reduceDvd, Nat.mod_mod_of_dvd, Bool.false_eq]
+        rw [(by decide : 16 = 2^4), Nat.testBit_mod_two_pow,
+          Bool.and_eq_false_eq_eq_false_or_eq_false]
+        left
+        simp only [decide_eq_false_iff_not, not_lt]
+        omega
+    . rw [hmin]; omega
+    . rw [hmin, Nat.mod_eq_of_lt] <;> omega
+  replace hsample_bits_slice : sample_bits_slice < 16 := by
+    rw [hsample_bits_slice]
+    exact Nat.lt_succ_of_le Nat.and_le_right
+  clear hBytesToBits
+  revert s_B_byte
+  revert sample_bits_slice
+  brute
+
+theorem Target2.samplePolyCBD.eta2_loop.spec.aux7 {s : samplePolyCBDState}
+  (BVector : Vector Byte (64 * ↑s.η))
+  (hBVector : BVector = ⟨s.B.take (64 * s.η), by have := s.hB; simp; omega⟩)
+  (hs1 : ∀ j < s.i, s.pe_dst[j]! = (Target.samplePolyCBD BVector)[j]!) (hs2 : ∀ j < 256, s.i ≤ j → s.pe_dst[j]! = 0)
+  (hs3 : s.src_i * 8 = s.i * 4) (hs4 : 8 ∣ s.i) (hs5 : 4 ∣ s.src_i) (hη : s.η.val = 2)
+  (hs6 : s.i < ↑key.MLWE_POLYNOMIAL_COEFFICIENTS) (j : ℕ) (hj1 : j < s.i + 8) (hj2 : ¬j < s.i)
+  (sample_bits : BitVec (8 * (List.slice s.src_i (s.src_i + 4) s.B.toList).length))
+  (hsample_bits :
+    sample_bits =
+      (BitVec.fromLEBytes (List.slice s.src_i (s.src_i + 4) s.B.toList) &&&
+          1431655765#(8 * (List.slice s.src_i (s.src_i + 4) s.B.toList).length)) +
+        (BitVec.fromLEBytes (List.slice s.src_i (s.src_i + 4) s.B.toList) >>> 1 &&&
+          1431655765#(8 * (List.slice s.src_i (s.src_i + 4) s.B.toList).length)))
+  (hBytesToBits : ∀ i < 64 * s.η.val, ∀ j < 8, (Target.bytesToBits BVector)[8 * i + j]! = s.B[i]!.testBit j)
+  (hj3 : j = s.i + 7) :
+  (↑↑(inner_loop.next_coefficient s.i 7
+      (inner_loop.next_coefficient s.i 6
+      (inner_loop.next_coefficient s.i 5
+      (inner_loop.next_coefficient s.i 4
+      (inner_loop.next_coefficient s.i 3
+      (inner_loop.next_coefficient s.i 2
+      (inner_loop.next_coefficient s.i 1
+      (inner_loop.next_coefficient s.i 0 (BitVec.setWidth 32 sample_bits)).1).1).1).1).1).1).1).2 : ZMod 3329) =
+    ∑ x : Fin s.η.val, ↑(Target.bytesToBits BVector)[2 * (s.i + 7) * ↑s.η + ↑x]!.toNat -
+      ∑ x : Fin s.η.val, ↑(Target.bytesToBits BVector)[2 * (s.i + 7) * ↑s.η + ↑s.η + ↑x]!.toNat := by
+  simp only [hη, Nat.mul_assoc 2 (s.i + 7) 2, Nat.mul_comm (s.i + 7) 2, ← Nat.mul_assoc 2 2 (s.i + 7),
+    Nat.reduceMul, Nat.mul_add 4, Nat.mul_comm 4 s.i, ← hs3, Fin.unfold2, Nat.mul_comm s.src_i 8]
+  conv in 8 * s.src_i + 28 + 0 => rw [(by omega : 8 * s.src_i + 28 + 0 = 8 * (s.src_i + 3) + 4)]
+  conv in 8 * s.src_i + 28 + 1 => rw [(by omega : 8 * s.src_i + 28 + 1 = 8 * (s.src_i + 3) + 5)]
+  conv in 8 * s.src_i + 28 + 2 + 0 => rw [(by omega : 8 * s.src_i + 28 + 2 + 0 = 8 * (s.src_i + 3) + 6)]
+  conv in 8 * s.src_i + 28 + 2 + 1 => rw [(by omega : 8 * s.src_i + 28 + 2 + 1 = 8 * (s.src_i + 3) + 7)]
+  rw [hBytesToBits (s.src_i + 3) (by scalar_tac) 4 (by omega),
+      hBytesToBits (s.src_i + 3) (by scalar_tac) 5 (by omega),
+      hBytesToBits (s.src_i + 3) (by scalar_tac) 6 (by omega),
+      hBytesToBits (s.src_i + 3) (by scalar_tac) 7 (by omega)]
+  unfold inner_loop.next_coefficient
+  simp only [BitVec.ofNat_eq_ofNat, ntt.Q.eq, UScalar.ofNat_val_eq, Nat.cast_ofNat, Nat.reduceAdd,
+    BitVec.toNat_add, BitVec.toNat_sub, Nat.reducePow, BitVec.toNat_ushiftRight, BitVec.toNat_and,
+    BitVec.toNat_setWidth, BitVec.toNat_ofNat, Nat.reduceMod, Nat.mod_add_mod, ← Nat.shiftRight_add]
+  olet hsample_bits_slice : sample_bits_slice := (sample_bits.toNat % 4294967296) >>> 28 &&& 15
+  olet hs_B_byte : s_B_byte := s.B[s.src_i + 3]!
+  replace hs_B_byte : sample_bits_slice = ((s_B_byte >>> 4) &&& 5) + ((s_B_byte >>> 5) &&& 5) := by
+    rw [hsample_bits_slice, hsample_bits]
+    simp only [BitVec.toNat_add, BitVec.toNat_and, BitVec.toNat_ofNat,
+      BitVec.toNat_ushiftRight, Nat.mod_add_mod, BitVec.natCast_eq_ofNat, BitVec.ofNat_and,
+      Nat.cast_ofNat, BitVec.ofNat_eq_ofNat]
+    have sHB := s.hB
+    have hmin : min (s.B.size - s.src_i) 4 = 4 := by scalar_tac
+    simp only [List.slice_length, Array.length_toList, add_tsub_cancel_left]
+    olet hy : y := (BitVec.fromLEBytes (List.slice s.src_i (s.src_i + 4) s.B.toList)).toNat >>> 1
+    olet hx : x := (BitVec.fromLEBytes (List.slice s.src_i (s.src_i + 4) s.B.toList)).toNat
+    olet hx' : x' := (x &&& 1431655765 % 2 ^ (8 * min (s.B.size - s.src_i) 4))
+    olet hy' : y' := (y &&& 1431655765 % 2 ^ (8 * min (s.B.size - s.src_i) 4))
+    rw [Nat.mod_eq_of_lt] at hx' hy' <;> (try rw [hmin]; decide +native)
+    have hy'' : y' < 1431655765 + 1 := by
+      apply Nat.lt_succ_of_le
+      rw [hy']
+      exact Nat.and_le_right
+    have hx'' : x' < 1431655765 + 1 := by
+      apply Nat.lt_succ_of_le
+      rw [hx']
+      exact Nat.and_le_right
+    rw [Nat.mod_eq_of_lt, Nat.mod_eq_of_lt]
+    . rw [(by decide : 15#8 = 2#8^4 - 1#8), BitVec.and_two_pow_sub_one_eq_mod]
+      ext k hk1
+      by_cases hk2 : k < 4
+      . simp only [← BitVec.getElem!_eq_getElem, BitVec.getElem!_mod_pow2_eq _ _ _ hk2,
+          BitVec.getElem!_eq_testBit_toNat, BitVec.toNat_ofNat, Nat.reducePow, BitVec.toNat_add,
+          BitVec.toNat_and, Nat.reduceMod, BitVec.toNat_ushiftRight, Nat.mod_add_mod]
+        rw [testBitMod256 ((x' + y') >>> 28) k (by omega), Nat.mod_eq_of_lt]
+        . rw [hx', hy', hy, shiftDistribMask1431655765 (by omega) hk2, ← hy, ← hy', ← hx']
+          apply testBitOfAdd 4 _ _ k hk2
+          . intro i hi
+            simp only [hx', hx, Nat.testBit_shiftRight, Nat.testBit_and,
+              ← BitVec.getElem!_eq_testBit_toNat, BitVec.fromLEBytes_getElem!]
+            rw [List.getElem!_slice, hs_B_byte, Array.getElem!_toList]
+            . rw [(by omega : (28 + i) / 8 = 3), (by omega : (28 + i) % 8 = 4 + i)]
+              simp_scalar
+              congr 1
+              revert i
+              decide
+            . scalar_tac
+          . intro i hi
+            simp only [hy', hy, hx, Nat.testBit_and, Nat.testBit_shiftRight,
+              ← BitVec.getElem!_eq_testBit_toNat, BitVec.fromLEBytes_getElem!]
+            by_cases hi2 : i < 3
+            . rw [(by omega : (1 + (28 + i)) / 8 = 3), (by omega : (1 + (28 + i)) % 8 = 5 + i),
+                List.getElem!_slice, hs_B_byte, Array.getElem!_toList]
+              . congr 1
+                revert i
+                decide
+              . scalar_tac
+            . have h1 : Nat.testBit 1431655765 (28 + i) = false := by revert i; decide
+              have h2 : Nat.testBit 5 i = false := by revert i; decide
+              simp only [h1, Bool.and_false, h2]
+        . have : (BitVec.toNat s_B_byte >>> 4) &&& 5 ≤ 5 := Nat.and_le_right
+          have : (BitVec.toNat s_B_byte >>> 5) &&& 5 ≤ 5 := Nat.and_le_right
+          omega
+      . have : (s_B_byte >>> 4 &&& 5#8) + (s_B_byte >>> 5 &&& 5#8) < 2^4 := by
+          clear hs_B_byte hBytesToBits
+          revert s_B_byte
+          decide +native -- **TODO** Once `brute` supports unbounded UScalars, `brute` should be faster
+        rw [← BitVec.getElem!_eq_getElem, ← BitVec.getElem!_eq_getElem,
+          BitVec.getElem!_mod_pow2_false _ _ _ (by omega), BitVec.getElem!_eq_testBit_toNat,
+          ← Nat.mod_eq_of_lt this]
+        simp only [BitVec.toNat_add, BitVec.toNat_and, BitVec.toNat_ofNat, Nat.reducePow,
+          Nat.reduceMod, BitVec.toNat_ushiftRight, Nat.mod_add_mod, BitVec.ofNat_eq_ofNat,
+          BitVec.toNat_pow, Nat.reduceDvd, Nat.mod_mod_of_dvd, Bool.false_eq]
+        rw [(by decide : 16 = 2^4), Nat.testBit_mod_two_pow,
+          Bool.and_eq_false_eq_eq_false_or_eq_false]
+        left
+        simp only [decide_eq_false_iff_not, not_lt]
+        omega
+    . rw [hmin]; omega
+    . rw [hmin, Nat.mod_eq_of_lt] <;> omega
+  replace hsample_bits_slice : sample_bits_slice < 16 := by
+    rw [hsample_bits_slice]
+    exact Nat.lt_succ_of_le Nat.and_le_right
+  clear hBytesToBits
+  revert s_B_byte
+  revert sample_bits_slice
+  brute
+
 def Target2.samplePolyCBD.eta2_loop.spec {s : Target2.samplePolyCBDState}
   (BVector : Vector Byte (64 * s.η))
   (hBVector : BVector = ⟨s.B.take (64 * s.η), by have := s.hB; simp; omega⟩)
@@ -66,7 +1019,7 @@ def Target2.samplePolyCBD.eta2_loop.spec {s : Target2.samplePolyCBDState}
       . rw [eta2_loop.inner_loop.preserves_below]
         . exact hs1 j hj2
         . exact hj2
-      . next hs4 =>
+      . next hs6 =>
         olet hsample_bits : sample_bits :=
           ((BitVec.fromLEBytes (List.slice s.src_i (s.src_i + 4) s.B.toList) &&&
               1431655765#(8 * (List.slice s.src_i (s.src_i + 4) s.B.toList).length)) +
@@ -88,14 +1041,34 @@ def Target2.samplePolyCBD.eta2_loop.spec {s : Target2.samplePolyCBDState}
         have hj3 : j = s.i ∨ j = s.i + 1 ∨ j = s.i + 2 ∨ j = s.i + 3 ∨
                    j = s.i + 4 ∨ j = s.i + 5 ∨ j = s.i + 6 ∨ j = s.i + 7 := by omega
         rcases hj3 with hj3 | hj3 | hj3 | hj3 | hj3 | hj3 | hj3 | hj3
-        . sorry
-        . sorry
-        . sorry
-        . sorry
-        . sorry
-        . sorry
-        . sorry
-        . sorry
+        . rw [hj3, Vector.getElem!_set!_ne (by omega), Vector.getElem!_set!_ne (by omega),
+            Vector.getElem!_set!_ne (by omega), Vector.getElem!_set!_ne (by omega),
+            Vector.getElem!_set!_ne (by omega), Vector.getElem!_set!_ne (by omega),
+            Vector.getElem!_set!_ne (by omega), Vector.getElem!_set! (by scalar_tac)]
+          apply eta2_loop.spec.aux0 <;> assumption
+        . rw [hj3, Vector.getElem!_set!_ne (by omega), Vector.getElem!_set!_ne (by omega),
+            Vector.getElem!_set!_ne (by omega), Vector.getElem!_set!_ne (by omega),
+            Vector.getElem!_set!_ne (by omega), Vector.getElem!_set!_ne (by omega),
+            Vector.getElem!_set! (by scalar_tac)]
+          apply eta2_loop.spec.aux1 <;> assumption
+        . rw [hj3, Vector.getElem!_set!_ne (by omega), Vector.getElem!_set!_ne (by omega),
+            Vector.getElem!_set!_ne (by omega), Vector.getElem!_set!_ne (by omega),
+            Vector.getElem!_set!_ne (by omega), Vector.getElem!_set! (by scalar_tac)]
+          apply eta2_loop.spec.aux2 <;> assumption
+        . rw [hj3, Vector.getElem!_set!_ne (by omega), Vector.getElem!_set!_ne (by omega),
+            Vector.getElem!_set!_ne (by omega), Vector.getElem!_set!_ne (by omega),
+            Vector.getElem!_set! (by scalar_tac)]
+          apply eta2_loop.spec.aux3 <;> assumption
+        . rw [hj3, Vector.getElem!_set!_ne (by omega), Vector.getElem!_set!_ne (by omega),
+            Vector.getElem!_set!_ne (by omega), Vector.getElem!_set! (by scalar_tac)]
+          apply eta2_loop.spec.aux4 <;> assumption
+        . rw [hj3, Vector.getElem!_set!_ne (by omega), Vector.getElem!_set!_ne (by omega),
+            Vector.getElem!_set! (by scalar_tac)]
+          apply eta2_loop.spec.aux5 <;> assumption
+        . rw [hj3, Vector.getElem!_set!_ne (by omega), Vector.getElem!_set! (by scalar_tac)]
+          apply eta2_loop.spec.aux6 <;> assumption
+        . rw [hj3, Vector.getElem!_set! (by scalar_tac)]
+          apply eta2_loop.spec.aux7 <;> assumption
     . intro j hj1 hj2
       simp only at hj2
       simp only [ReduceZMod.reduceZMod]
