proofs/Symcrust/Properties/SamplePolyCBD/Target2HelperLemmas.lean
@@ -1,0 +1,29 @@
+import Symcrust.Spec
+import Symcrust.Code.Funs
+import Symcrust.Brute
+import Symcrust.Properties.SamplePolyCBD.Target2Code
+
+/-!
+This file contains helper lemmas that are used in both `Target2Eta2Proofs.lean` and `Target2Eta3Proofs.lean`
+-/
+
+#setup_aeneas_simps
+
+namespace Symcrust.SpecAux
+
+open Symcrust.Spec
+open Aeneas Aeneas.Std Aeneas.SRRange
+
+set_option maxHeartbeats 1000000
+
+lemma testBitMod256 (a k : ℕ) (hk : k < 6) : (a % 256).testBit k = a.testBit k := by
+  have hk2 : decide (k < 6) := by simp [hk]
+  rw [← Nat.testBit_two_pow_sub_one] at hk2
+  rw [← Bool.and_true (a.testBit k), ← hk2, ← Nat.testBit_and, (by decide : 256 = 2^8),
+    Nat.testBit_mod_two_pow]
+  simp_scalar
+  simp [hk2]
+
+lemma testBitOfAdd {x1 x2 y1 y2 : ℕ} (n : ℕ) (hx : ∀ i < n, x1.testBit i = x2.testBit i)
+  (hy : ∀ i < n, y1.testBit i = y2.testBit i) : ∀ i < n, (x1 + y1).testBit i = (x2 + y2).testBit i := by
+  sorry
